crates/synch-verified/lean/VerifiedCore/Commands/Generated.lean
@@ -239,7 +239,7 @@ instance : Decode Cas.Receive.ProvenSubtree where
 
 instance : Encode Cas.Project.Blob where
   encode out value := match value with
-    | .mk a0 a1 a2 a3 a4 a5 a6 a7 => out |>.put a0 |>.put a1 |>.put a2 |>.put a3 |>.put a4 |>.put a5 |>.put a6 |>.put a7
+    | .mk a0 a1 a2 a3 a4 a5 a6 a7 a8 a9 => out |>.put a0 |>.put a1 |>.put a2 |>.put a3 |>.put a4 |>.put a5 |>.put a6 |>.put a7 |>.put a8 |>.put a9
 
 instance : Decode Cas.Project.Blob where
   decode := do
@@ -251,7 +251,9 @@ instance : Decode Cas.Project.Blob where
     let a5 ← Decode.decode
     let a6 ← Decode.decode
     let a7 ← Decode.decode
-    return .mk a0 a1 a2 a3 a4 a5 a6 a7
+    let a8 ← Decode.decode
+    let a9 ← Decode.decode
+    return .mk a0 a1 a2 a3 a4 a5 a6 a7 a8 a9
 
 instance : Encode Cas.Project.Summary where
   encode out value := match value with
@@ -641,6 +643,7 @@ instance : Encode Commands.Command where
     | .planExchange a0 a1 a2 => out.push 45 |>.put a0 |>.put a1 |>.put a2
     | .trieFetch a0 a1 a2 a3 a4 a5 a6 a7 a8 => out.push 46 |>.put a0 |>.put a1 |>.put a2 |>.put a3 |>.put a4 |>.put a5 |>.put a6 |>.put a7 |>.put a8
     | .trieNormalize a0 => out.push 47 |>.put a0
+    | .casBlobIn a0 a1 => out.push 48 |>.put a0 |>.put a1
 
 instance : Decode Commands.Command where
   decode := do
@@ -693,6 +696,7 @@ instance : Decode Commands.Command where
     | 45 => return .planExchange (← Decode.decode) (← Decode.decode) (← Decode.decode)
     | 46 => return .trieFetch (← Decode.decode) (← Decode.decode) (← Decode.decode) (← Decode.decode) (← Decode.decode) (← Decode.decode) (← Decode.decode) (← Decode.decode) (← Decode.decode)
     | 47 => return .trieNormalize (← Decode.decode)
+    | 48 => return .casBlobIn (← Decode.decode) (← Decode.decode)
     | _ => throw ()
 
 end VerifiedCore
